lean/Main.lean
@@ -14,10 +14,8 @@ local notation "Variable" => Variable (τ := SimpleType)
 
 def runFlowAnalysis (s : Stmt) : LoweredExpr ⊕ String :=
   let loweredResult := do
-    -- TODO: labels should identify the program point at which each value comes into existence, but
-    -- the syntax doesn't yet carry enough information to do that, so every value currently has the
-    -- version `ValueVersion.unspecified`.  Until that changes, a single label suffices.
-    let runResult ← elabStmtImpl (ℓ := Unit) s ⟨⟩ AlgState.initial
+    -- `s` is the root of the syntax tree, so its AST path is `[]`.
+    let runResult ← elabStmtImpl s ⟨[]⟩ AlgState.initial
     pure runResult.fst
   match loweredResult with
     | .ok m => .inl m
